Implement a step-indexed normalization function.

theories/NormalForms.v
@@ -1,7 +1,7 @@
 (** * LogRel.NormalForms: definition of normal and neutral forms, and properties. *)
 From Coq Require Import ssrbool.
 From LogRel.AutoSubst Require Import core unscoped Ast Extra.
-From LogRel Require Import Utils BasicAst Context Closed.
+From LogRel Require Import Utils BasicAst Context Closed Computation.
 
 (** Deep normal forms *)
 
@@ -339,3 +339,118 @@ Section RenWhnf.
 End RenWhnf.
 
 #[global] Hint Resolve whne_ren whnf_ren isType_ren isPosType_ren isFun_ren isCanonical_ren : gen_typing.
+
+(** Computational variant of the above *)
+
+Fixpoint is_nf ne t {struct t} := match t with
+| tSort _ | tNat | tZero | tEmpty => negb ne
+| tProd A B => negb ne && is_nf false A && is_nf false B
+| tLambda A t => negb ne && is_nf false A && is_nf false t
+| tSucc t => negb ne && is_nf false t
+| tSig A B => negb ne && is_nf false A && is_nf false B
+| tPair A B a b => negb ne && is_nf false A && is_nf false B && is_nf false a && is_nf false b
+| tId A t u => negb ne && is_nf false A && is_nf false t && is_nf false u
+| tRefl A t => negb ne && is_nf false A && is_nf false t
+| tRel _ => true
+| tApp t u => is_nf true t && is_nf false u
+| tNatElim P hz hs n => is_nf false P && is_nf false hz && is_nf false hs && is_nf true n
+| tEmptyElim P e => is_nf false P && is_nf true e
+| tFst t => is_nf true t
+| tSnd t => is_nf true t
+| tIdElim A x P hr y e =>
+  is_nf false A && is_nf false x && is_nf false P && is_nf false hr && is_nf false y && is_nf true e
+| tQuote t => is_nf false t && negb (is_closedn 0 t)
+end.
+
+Definition is_dnf t := is_nf false t.
+Definition is_dne t := is_nf true t.
+
+Fixpoint is_wnf ne t {struct t} := match t with
+| tSort _ | tNat | tZero | tEmpty => negb ne
+| tProd A B => negb ne
+| tLambda A t => negb ne
+| tSucc t => negb ne
+| tSig A B => negb ne
+| tPair A B a b => negb ne
+| tId A t u => negb ne
+| tRefl A t => negb ne
+| tRel _ => true
+| tApp t u => is_wnf true t
+| tNatElim P hz hs n => is_wnf true n
+| tEmptyElim P e => is_wnf true e
+| tFst t => is_wnf true t
+| tSnd t => is_wnf true t
+| tIdElim A x P hr y e => is_wnf true e
+| tQuote t => is_dnf t && negb (is_closedn 0 t)
+end.
+
+Definition is_whnf t := is_wnf false t.
+Definition is_whne t := is_wnf true t.
+
+Lemma is_nf_incl : forall t, is_dne t -> is_dnf t.
+Proof.
+induction t; cbn; intros.
+all: repeat match goal with H : _ |- _ => apply andb_prop in H; destruct H end.
+all: repeat (apply andb_true_intro; split); eauto.
+Qed.
+
+Lemma dnf_dne_is_nf :
+  (forall t, dnf t -> is_dnf t = true) × (forall t, dne t -> is_dne t = true).
+Proof.
+apply dnf_dne_rect; cbn; intros.
+all: repeat (apply andb_true_intro; split); eauto.
++ now apply is_nf_incl.
++ now apply Bool.eq_true_not_negb.
+Qed.
+
+Lemma is_nf_dnf_dne :
+  forall t, (is_dnf t = true -> dnf t) × (is_dne t = true -> dne t).
+Proof.
+induction t; split; intros; cbn in *.
+all: repeat match goal with H : _ × _ |- _ => destruct H end.
+all: repeat match goal with H : _ |- _ => apply andb_prop in H; destruct H end.
+all: try discriminate.
+all: try match goal with |- dnf _ => constructor end.
+all: try match goal with |- dne _ => constructor end.
+all: eauto using dnf, dne.
++ now eapply contraNnot.
++ now eapply contraNnot.
+Qed.
+
+Lemma is_dnf_dnf : forall t, is_dnf t = true -> dnf t.
+Proof.
+intros; now eapply is_nf_dnf_dne.
+Qed.
+
+Lemma dnf_is_dnf : forall t, dnf t -> is_dnf t = true.
+Proof.
+intros; now eapply dnf_dne_is_nf.
+Qed.
+
+Lemma is_dne_dne : forall t, is_dne t = true -> dne t.
+Proof.
+intros; now eapply is_nf_dnf_dne.
+Qed.
+
+Lemma dne_is_dne : forall t, dne t -> is_dne t = true.
+Proof.
+intros; now eapply dnf_dne_is_nf.
+Qed.
+
+Lemma whne_is_whne : forall t, whne t -> is_whne t = true.
+Proof.
+induction 1; cbn.
+all: repeat (apply andb_true_intro; split); eauto using whne, whnf.
++ now eapply dnf_dne_is_nf.
++ apply Bool.eq_true_not_negb; tea.
+Qed.
+
+Lemma is_whne_whne : forall t, is_whne t = true -> whne t.
+Proof.
+induction t; cbn; intros; try discriminate.
+all: repeat match goal with H : _ |- _ => apply andb_prop in H; destruct H end.
+all: eauto using whne, whnf.
++ constructor.
+  - unfold closed0; destruct is_closedn; cbn in *; congruence.
+  - now apply is_nf_dnf_dne.
+Qed.
